pset4

Lab4Sol.v
@@ -6,11 +6,10 @@ Require Import Frap.
 (* Authors: Peng Wang (wangpeng@csail.mit.edu), Adam Chlipala (adamc@csail.mit.edu) *)
 
 
-(** Challenge 1: Nondeterminism *)
+(** * Challenge 1: Nondeterminism *)
 
 Module Challenge1.
-
-  (* Here's the same old arithmetic-expression language. *)  
+  
   Inductive arith : Set :=
   | Const (n : nat)
   | Var (x : var)
@@ -18,7 +17,6 @@ Module Challenge1.
   | Minus (e1 e2 : arith)
   | Times (e1 e2 : arith).
 
-  (* And here's the same old command language, with one twist. *)
   Inductive cmd :=
   | Skip
   | Assign (x : var) (e : arith)
@@ -27,11 +25,6 @@ Module Challenge1.
   | While (e : arith) (body : cmd)
   | Choice (c1 c2 : cmd).
 
-  (* The last construct [Choice c1 c2] stands for a *nondeterministic choice* at
-   * runtime.  Every time we reach this command, we may run either [c1] or [c2]
-   * (but not both). *)
-
-  (* Same old expression evaluation *)
   Definition valuation := fmap var nat.
   Fixpoint interp (e : arith) (v : valuation) : nat :=
     match e with
@@ -45,9 +38,6 @@ Module Challenge1.
     | Minus e1 e2 => interp e1 v - interp e2 v
     | Times e1 e2 => interp e1 v * interp e2 v
     end.
-
-  (* THE CHALLENGE IS: update each semantics with appropriate rules for
-   * [Choice] and update the proofs below. *)
 
   (** Big-step semantics *)
 
@@ -81,7 +71,7 @@ Module Challenge1.
       -> eval v (Choice c1 c2) v'
   | EvalChoice2 : forall v c1 c2 v',
       eval v c2 v'
-      -> eval v (Choice c1 c2) v'. 
+      -> eval v (Choice c1 c2) v'.
 
   (** Small-step semantics *)
 
@@ -109,13 +99,12 @@ Module Challenge1.
       step (v, Choice c1 c2) (v, c1)
   | StepChoice2 : forall v c1 c2,
       step (v, Choice c1 c2) (v, c2).
-                                  
 
   Hint Constructors trc step eval.
 
   Lemma step_star_Seq : forall v c1 c2 v' c1',
-    step^* (v, c1) (v', c1')
-    -> step^* (v, Sequence c1 c2) (v', Sequence c1' c2).
+      step^* (v, c1) (v', c1')
+      -> step^* (v, Sequence c1 c2) (v', Sequence c1' c2).
   Proof.
     induct 1; eauto.
     cases y; eauto.
@@ -124,28 +113,26 @@ Module Challenge1.
   Hint Resolve step_star_Seq.
 
   Theorem big_small : forall v c v', eval v c v'
-    -> step^* (v, c) (v', Skip).
+                                     -> step^* (v, c) (v', Skip).
   Proof.
     induct 1; eauto 6 using trc_trans.
   Qed.
 
-  Lemma small_big'' : forall v c v' c',
-      step (v, c) (v', c')
-      -> forall v'', eval v' c' v''
-                     -> eval v c v''.
+  Lemma small_big'' : forall v c v' c', step (v, c) (v', c')
+                                        -> forall v'', eval v' c' v''
+                                                       -> eval v c v''.
   Proof.
     induct 1; simplify;
-    repeat match goal with
-           | [ H : eval _ _ _ |- _ ] => invert1 H
-           end; eauto.
+      repeat match goal with
+             | [ H : eval _ _ _ |- _ ] => invert1 H
+             end; eauto.
   Qed.
 
   Hint Resolve small_big''.
 
-  Lemma small_big' : forall v c v' c',
-      step^* (v, c) (v', c')
-      -> forall v'', eval v' c' v''
-                     -> eval v c v''.
+  Lemma small_big' : forall v c v' c', step^* (v, c) (v', c')
+                                         -> forall v'', eval v' c' v''
+                                                  -> eval v c v''.
   Proof.
     induct 1; eauto.
     cases y; eauto.
@@ -153,9 +140,8 @@ Module Challenge1.
 
   Hint Resolve small_big'.
 
-  Theorem small_big : forall v c v',
-      step^* (v, c) (v', Skip)
-      -> eval v c v'.
+  Theorem small_big : forall v c v', step^* (v, c) (v', Skip)
+                                     -> eval v c v'.
   Proof.
     eauto.
   Qed.
@@ -188,7 +174,11 @@ Module Challenge1.
       -> step0 (v, While e body) (v, Sequence body (While e body))
   | Step0WhileFalse : forall v e body,
       interp e v = 0
-      -> step0 (v, While e body) (v, Skip).
+      -> step0 (v, While e body) (v, Skip)
+  | Step0Choice1 : forall v c1 c2,
+      step0 (v, Choice c1 c2) (v, c1)
+  | Step0Choice2 : forall v c1 c2,
+      step0 (v, Choice c1 c2) (v, c2).
 
   Inductive cstep : valuation * cmd -> valuation * cmd -> Prop :=
   | CStep : forall C v c v' c' c1 c2,
@@ -200,19 +190,17 @@ Module Challenge1.
   Hint Constructors plug step0 cstep.
 
   Theorem step_cstep : forall v c v' c',
-    step (v, c) (v', c')
-    -> cstep (v, c) (v', c').
+      step (v, c) (v', c')
+      -> cstep (v, c) (v', c').
   Proof.
     induct 1; repeat match goal with
                      | [ H : cstep _ _ |- _ ] => invert H
                      end; eauto.
   Qed.
 
-  Hint Resolve step_cstep.
-
   Lemma step0_step : forall v c v' c',
-    step0 (v, c) (v', c')
-    -> step (v, c) (v', c').
+      step0 (v, c) (v', c')
+      -> step (v, c) (v', c').
   Proof.
     induct 1; eauto.
   Qed.
@@ -220,10 +208,10 @@ Module Challenge1.
   Hint Resolve step0_step.
 
   Lemma cstep_step' : forall C c0 c,
-    plug C c0 c
-    -> forall v' c'0 v c', step0 (v, c0) (v', c'0)
-    -> plug C c'0 c'
-    -> step (v, c) (v', c').
+      plug C c0 c
+      -> forall v' c'0 v c', step0 (v, c0) (v', c'0)
+                       -> plug C c'0 c'
+                       -> step (v, c) (v', c').
   Proof.
     induct 1; simplify; repeat match goal with
                                | [ H : plug _ _ _ |- _ ] => invert1 H
@@ -233,8 +221,8 @@ Module Challenge1.
   Hint Resolve cstep_step'.
 
   Theorem cstep_step : forall v c v' c',
-    cstep (v, c) (v', c')
-    -> step (v, c) (v', c').
+      cstep (v, c) (v', c')
+      -> step (v, c) (v', c').
   Proof.
     induct 1; eauto.
   Qed.
@@ -242,10 +230,7 @@ Module Challenge1.
 End Challenge1.
 
 
-(** Challenge 2: Functions and Control Stack *)
-
-(* This time, we give you the new semantics and ask you to fill in the
- * proofs. *)
+(** * Challenge 2: Functions and Control Stack *)
 
 Module Challenge2.
   
@@ -258,24 +243,15 @@ Module Challenge2.
 
   Definition valuation := fmap var nat.
   
-  (* The new twist this time: function calls! *)
   Inductive cmd :=
   | Skip
   | Assign (x : var) (e : arith)
   | Sequence (c1 c2 : cmd)
   | If (e : arith) (then_ else_ : cmd)
   | While (e : arith) (body : cmd)
-
   | Call (lhs f : var) (arg : arith)
-  (* Calling the function named [f] with the argument [arg], assigning the
-   * return value to [lhs] *)
-
-  | InCall (v : valuation) (lhs ret : var) (c : cmd).
-  (* This other command form only arises in the course of small-step evaluation.
-   * It means that a call to a function was made from a context with valuation
-   * [v], waiting to assign the return value to variable [lhs].  In the called
-   * function, variable [ret] is assigned to hold the return value, and we have
-   * executed that function up to command [c]. *)
+  | InCall (v : valuation) (lhs ret : var) (c : cmd)
+  | Return (e : arith).
 
   Fixpoint interp (e : arith) (v : valuation) : nat :=
     match e with
@@ -290,14 +266,14 @@ Module Challenge2.
     | Times e1 e2 => interp e1 v * interp e2 v
     end.
 
-  (* Every function in the program is mapped to one of these. *)
+  (* function specification *)
   Record fun_spec := {
-    Arg : var; (* Name of formal parameter *)
-    Ret : var; (* Variable where return value must be stored *)
-    Body : cmd (* Body to execute upon call *)
+    Arg : var;
+    Ret : var;
+    Body : cmd
   }.
 
-  (** An environment is a mapping from function names to function specs. *)
+  (** An environment is a mapping from function names to function specs *)
   Definition environment := fmap var fun_spec.
 
   Section env.
@@ -330,23 +306,13 @@ Module Challenge2.
     | EvalWhileFalse : forall v e body,
         interp e v = 0
         -> eval v (While e body) v
-
     | EvalCall : forall v lhs f arg spec v',
         env $? f = Some spec 
-        (* When making a function call, look up the function spec by name. *)
-
         -> eval ($0 $+ (spec.(Arg), interp arg v)) spec.(Body) v'
-        (* Then evaluate the callee's body, in a valuation with just the actual
-         * parameter value. *)
-
         -> eval v (Call lhs f arg) (v $+ (lhs, interp (Var spec.(Ret)) v'))
-        (* Extend the original valuation with the function return value. *)
-
     | EvalInCall : forall v0 lhs ret v c v',
         eval v c v'
         -> eval v (InCall v0 lhs ret c) (v0 $+ (lhs, interp (Var ret) v')).
-        (* This [InCall] case is just to make the proofs below go through nicely.
-         * We don't actually need [InCall] for big-step evaluation. *)
 
     (** Small-step semantics *)
 
@@ -370,44 +336,104 @@ Module Challenge2.
     | StepWhileFalse : forall v e body,
         interp e v = 0
         -> step (v, While e body) (v, Skip)
-
     | StepStartCall : forall v lhs f arg spec,
         env $? f = Some spec
         -> step (v, Call lhs f arg) ($0 $+ (spec.(Arg), interp arg v), InCall v lhs spec.(Ret) spec.(Body))
-        (* To begin with a function call, step to an [InCall], in a fresh
-         * valuation containing only the actual parameter value.  Remember the
-         * current valuation as an argument to [InCall]. *)
-
     | StepInCall : forall v c v' c' v0 lhs ret,
         step (v, c) (v', c')
         -> step (v, InCall v0 lhs ret c) (v', InCall v0 lhs ret c')
-        (* Basic congruence rule, for stepping with an [InCall], meaning that
-         * we take a step in the function that was called, leaving alone the
-         * "call stack" around it. *)
-
     | StepEndCall : forall v0 lhs ret v,
         step (v, InCall v0 lhs ret Skip) (v0, Assign lhs (Const (interp (Var ret) v))).
-        (* When does our [InCall] detour end?  When the callee's body has
-         * stepped to [Skip].  Then we back up and assign to the caller's
-         * variable that has been waiting to receive the return value. *)
 
+    Hint Constructors trc step eval.
+
+    Lemma step_star_Seq : forall v c1 c2 v' c1',
+        step^* (v, c1) (v', c1')
+        -> step^* (v, Sequence c1 c2) (v', Sequence c1' c2).
+    Proof.
+      induct 1; eauto.
+      cases y; eauto.
+    Qed.
+
+    Hint Resolve step_star_Seq.
+
+    Lemma step_star_InCall : forall v c v' c' v0 lhs ret,
+        step^* (v, c) (v', c')
+        -> step^* (v, InCall v0 lhs ret c) (v', InCall v0 lhs ret c').
+    Proof.
+      induct 1; eauto.
+      cases y; eauto.
+    Qed.
+
+    Hint Resolve step_star_InCall.
+    
     Theorem big_small : forall v c v',
         eval v c v'
         -> step^* (v, c) (v', Skip).
     Proof.
-    Admitted.
+      induct 1; simplify; eauto 4 using trc_trans.
+      {
+        econstructor.
+        eauto.
+        eapply trc_trans.
+        apply step_star_Seq.
+        eassumption.
+        eauto.
+      }
+      {
+        econstructor; eauto.
+        eapply trc_trans.
+        {
+          apply step_star_InCall.
+          eassumption.
+        }
+        eauto.
+      }
+      {
+        eapply trc_trans.
+        {
+          apply step_star_InCall.
+          eassumption.
+        }
+        eauto.
+      }
+    Qed.
+
+    Lemma small_big'' : forall v c v' c',
+        step (v, c) (v', c')
+        -> forall v'', eval v' c' v''
+                       -> eval v c v''.
+    Proof.
+      induct 1; simplify;
+        repeat match goal with
+               | [ H : eval _ _ _ |- _ ] => invert1 H
+               end; eauto.
+      {
+        econstructor; eauto.
+      }
+    Qed.
+
+    Hint Resolve small_big''.
+
+    Lemma small_big' : forall v c v' c',
+        step^* (v, c) (v', c')
+        -> forall v'', eval v' c' v''
+                       -> eval v c v''.
+    Proof.
+      induct 1; eauto.
+      cases y; eauto.
+    Qed.
+
+    Hint Resolve small_big'.
 
     Theorem small_big : forall v c v',
         step^* (v, c) (v', Skip)
         -> eval v c v'.
     Proof.
-    Admitted.
+      eauto.
+    Qed.
 
     (** Small-step semantics with control stack *)
-
-    (* As an alternative to evaluation contexts, we can also use an explicit
-     * representation of a call stack.  First, a basic step relation that
-     * doesn't need a call stack. *)
 
     Inductive step0 : valuation * cmd -> valuation * cmd -> Prop :=
     | Step0Assign : forall v x e,
@@ -425,73 +451,171 @@ Module Challenge2.
         interp e v = 0
         -> step0 (v, While e body) (v, Skip).
 
-    (* Our call stack will be a sequence of frames like these. *)
     Record frame := {
-      Val : valuation; (* Local variable values *)
-      Cont : cmd;      (* Command waiting to run after called function
-                        * returns *)
-      LHS : var;       (* Variable waiting to receive return value of called
-                        * function *)
-      RetVar : var     (* Place to store return value of this function *)
+      Val : valuation;
+      Cont : cmd;
+      LHS : var;
+      RetVar : var
     }.
 
     Definition stack := list frame.
 
-    (* What are the four components of states in this semantics?
-     * #1: call stack
-     * #2: local variables of topmost call
-     * #3: command to run next
-     * #4: additional command to run afterward, called the *continuation* *)
     Inductive stepcs : stack * valuation * cmd * cmd -> stack * valuation * cmd * cmd -> Prop :=
-
-    (* Easy case: just step the main command as usual *)
     | StepcsStep0 : forall v c v' c' s k,
         step0 (v, c) (v', c') ->
         stepcs (s, v, c, k) (s, v', c', k)
-
-    (* Fancier case: when encountering a sequence, pop off its second step and
-     * push it onto the front of the continuation. *)
     | StepcsSeq : forall s v c1 c2 k,
         stepcs (s, v, Sequence c1 c2, k) (s, v, c1, Sequence c2 k)
-
-    (* Natural companion to last rule: when the main command is empty, start
-     * running the next command of the continuation, if one is available. *)
     | StepcsCont : forall s v k1 k2,
         stepcs (s, v, Skip, Sequence k1 k2) (s, v, k1, k2)
-
-    (* When both the main command and the continuation are [Skip], we're done
-     * running this function.  Time to pop the call stack and return to the
-     * caller. *)
     | StepcsReturn : forall fr s v,
         stepcs (fr :: s, v, Skip, Skip) (s, fr.(Val) $+ (fr.(LHS), interp (Var fr.(RetVar)) v), Skip, fr.(Cont))
-
-    (* To make a cal, push a new frame onto the call stack. *)
     | StepcsCall : forall s v lhs f arg k spec,
         env $? f = Some spec
         -> stepcs (s, v, Call lhs f arg, k) ({| Val := v; Cont := k; LHS := lhs; RetVar := spec.(Ret)|} :: s, $0 $+ (spec.(Arg), interp arg v), spec.(Body), Skip)
-
-    (* We don't actually need [InCall] in this semantics, but here's a single
-     * step to get rid of it. *)
     | StepcsInCall : forall s v0 lhs ret v c k,
         stepcs (s, v, InCall v0 lhs ret c, k) ({| Val := v0; Cont := k; LHS := lhs; RetVar := ret|} :: s, v, c, Skip).
+    
+    Hint Constructors step0 stepcs.
+
+    Hint Extern 0 (_ <> _) => equality.
+
+    Lemma eval_stepcs' : forall v c v',
+        eval v c v'
+        -> forall s k, stepcs^* (s, v, c, k) (s, v', Skip, k).
+    Proof.
+      induct 1; simplify; eauto 4 using trc_trans.
+      {
+        econstructor; eauto.
+        econstructor; eauto.
+        eapply trc_trans; eauto.
+      }
+      {
+        econstructor; eauto.
+        eapply trc_trans; eauto.
+      }
+    Qed.
     
     Theorem eval_stepcs : forall v c v',
         eval v c v'
         -> stepcs^* ([], v, c, Skip) ([], v', Skip, Skip).
     Proof.
-    Admitted.
+      simplify.
+      eapply eval_stepcs'.
+      eauto.
+    Qed.
+
+    Definition unravel_frame c fr := Sequence (InCall fr.(Val) fr.(LHS) fr.(RetVar) c) fr.(Cont).
+    Arguments unravel_frame _ _ / .
+      
+    Definition unravel s c := fold_left unravel_frame s c.
+    Arguments unravel / .
+
+    Lemma eval_unravel : forall s v c v' c',
+        (forall v'', eval v' c' v'' -> eval v c v'') ->
+        forall v'',
+          eval v' (unravel s c') v'' ->
+          eval v (unravel s c) v''.
+    Proof.
+      induct s; simplify.
+      { eauto. }
+      eapply IHs; try eassumption.
+      simplify.
+      repeat match goal with
+             | [ H : eval _ _ _ |- _ ] => invert1 H
+             end; eauto.
+      econstructor; try eassumption.
+      eauto.
+    Qed.
+    
+    Lemma step0_eval : forall v c v' c',
+        step0 (v, c) (v', c')
+        -> forall v'', eval v' c' v''
+                       -> eval v c v''.
+    Proof.
+      induct 1; simplify;
+        repeat match goal with
+               | [ H : eval _ _ _ |- _ ] => invert1 H
+               end; eauto.
+    Qed.
+
+    Hint Resolve step0_eval.
+
+    Lemma stepcs_eval'' : forall s v c k s' v' c' k',
+        stepcs (s, v, c, k) (s', v', c', k')
+        -> forall v'', eval v' (unravel s' (Sequence c' k')) v''
+                       -> eval v (unravel s (Sequence c k)) v''.
+    Proof.
+      induct 1; simplify; eapply eval_unravel; try eassumption; simplify;
+        repeat match goal with
+               | [ H : eval _ _ _ |- _ ] => invert1 H
+               end; eauto 6.
+      {
+        econstructor; try eassumption.
+        econstructor; eauto.
+      }
+      {
+        econstructor; try eassumption.
+        econstructor; eauto.
+      }
+    Qed.
+
+    Hint Resolve stepcs_eval''.
+
+    Lemma stepcs_eval' : forall s v c k s' v' c' k',
+        stepcs^* (s, v, c, k) (s', v', c', k')
+        -> forall v'', eval v' (unravel s' (Sequence c' k')) v''
+                       -> eval v (unravel s (Sequence c k)) v''.
+    Proof.
+      induct 1; eauto.
+      repeat match goal with
+             | [ H : (_ * _)%type |- _ ] => cases H
+             end; eauto.
+    Qed.
+
+    Hint Resolve stepcs_eval'.
 
     Theorem stepcs_eval : forall v c v',
         stepcs^* ([], v, c, Skip) ([], v', Skip, Skip)
         -> eval v c v'.
     Proof.
-    Admitted.
+      simplify.
+      eapply stepcs_eval' in H; simplify;
+        repeat match goal with
+               | [ H : eval _ _ _ |- _ ] => invert1 H
+               end; eauto.
+    Qed.
+
 
   End env.
 
-End Challenge2.
+  (* Here's how to handle the [Return] command. *)
+  Module StrangeAlternateUniverse.
+    Section Return.
+      Variable env : environment.
 
-(* CHALLENGE #3: Extend the language with an explicit "return" command and add
- * one rule to the control-stack semantics to explain its effect.
- * The other semantics styles would need bigger modifications to handle
- * "return," so here we see an advantage of the control-stack formulation. *)
+      Inductive stepcs : stack * valuation * cmd * cmd -> stack * valuation * cmd * cmd -> Prop :=
+      | StepcsStep0 : forall v c v' c' s k,
+          step0 (v, c) (v', c') ->
+          stepcs (s, v, c, k) (s, v', c', k)
+      | StepcsSeq : forall s v c1 c2 k,
+          stepcs (s, v, Sequence c1 c2, k) (s, v, c1, Sequence c2 k)
+      | StepcsCont : forall s v k1 k2,
+          stepcs (s, v, Skip, Sequence k1 k2) (s, v, k1, k2)
+      | StepcsReturn : forall fr s v,
+          stepcs (fr :: s, v, Skip, Skip) (s, fr.(Val) $+ (fr.(LHS), interp (Var fr.(RetVar)) v), Skip, fr.(Cont))
+
+      (****)
+      | StepcsExplicitReturn : forall fr s v e k,
+          stepcs (fr :: s, v, Return e, k) (s, fr.(Val) $+ (fr.(LHS), interp e v), Skip, fr.(Cont))
+      (****)
+
+      | StepcsCall : forall s v lhs f arg k spec,
+          env $? f = Some spec
+          -> stepcs (s, v, Call lhs f arg, k) ({| Val := v; Cont := k; LHS := lhs; RetVar := spec.(Ret)|} :: s, $0 $+ (spec.(Arg), interp arg v), spec.(Body), Skip)
+      | StepcsInCall : forall s v0 lhs ret v c k,
+          stepcs (s, v, InCall v0 lhs ret c, k) ({| Val := v0; Cont := k; LHS := lhs; RetVar := ret|} :: s, v, c, Skip).
+    End Return.
+  End StrangeAlternateUniverse.
+
+End Challenge2.
