pset3/Pset3Sol.v
@@ -1,0 +1,254 @@
+(** * 6.887 Formal Reasoning About Programs, Spring 2016 - Pset 3 *)
+
+Require Import Frap Pset3Sig.
+
+Set Implicit Arguments.
+
+
+(* Authors: Adam Chlipala (adamc@csail.mit.edu), Peng Wang (wangpeng@csail.mit.edu) *)
+
+
+Lemma assumptionsHold_sound : forall state prs (st : state) pm,
+    (forall x b, pm $? x = Some b
+               -> match prs $? x with
+                  | Some pr => pr st <-> b = true
+                  | None => False
+                  end)
+  -> forall asms, assumptionsHold pm asms = true
+  -> assumptionsAccurate prs asms st.
+Proof.
+  induct asms; simplify; propositional.
+
+  cases (assertionHolds pm a); simplify; try equality.
+  unfold assertionHolds, assertionAccurate in *.
+  cases a; simplify.
+  cases (pm $? AssumedPredicate); try equality.
+  cases b.
+  cases AssumedToBe; try equality.
+  apply H in Heq0.
+  cases (prs $? AssumedPredicate); propositional.
+  cases AssumedToBe; try equality.
+  apply H in Heq0.
+  cases (prs $? AssumedPredicate); propositional.
+  apply H.
+  assumption.
+
+  cases (assertionHolds pm a); simplify; equality.
+Qed.
+
+Lemma applyRule_sound : forall state (doIt : state -> state -> Prop)
+                               prs x b st st' r pm pm',
+  (forall x b, pm $? x = Some b
+               -> match prs $? x with
+                  | Some pr => pr st <-> b = true
+                  | None => False
+                  end)
+  -> (forall x b, pm' $? x = Some b
+                  -> match prs $? x with
+                     | Some pr => pr st' <-> b = true
+                     | None => False
+                     end)
+  -> applyRule pm pm' r $? x = Some b
+  -> ruleAccurate prs doIt r
+  -> doIt st st'
+  -> match prs $? x with
+     | Some pr => pr st' <-> b = true
+     | None => False
+     end.
+Proof.
+  unfold applyRule; simplify.
+  cases r.
+  cases (assumptionsHold pm Assumptions).
+  cases (AssumedToBe Conclusion).
+
+  cases (x ==v AssumedPredicate Conclusion); simplify.
+  invert H1.
+  unfold ruleAccurate in H2; simplify.
+  apply H2 in H3.
+  unfold assertionAccurate in H3.
+  rewrite Heq0 in H3.
+  cases (prs $? AssumedPredicate Conclusion); propositional.
+  eapply assumptionsHold_sound.
+  eassumption.
+  assumption.
+  apply H0; assumption.
+  
+  cases (x ==v AssumedPredicate Conclusion); simplify.
+  invert H1.
+  unfold ruleAccurate in H2; simplify.
+  apply H2 in H3.
+  unfold assertionAccurate in H3.
+  rewrite Heq0 in H3.
+  cases (prs $? AssumedPredicate Conclusion); propositional.
+  eapply assumptionsHold_sound.
+  eassumption.
+  assumption.
+  apply H0; assumption.
+
+  apply H0; assumption.
+Qed.
+
+Lemma applyRules_sound' : forall state (doIt : state -> state -> Prop)
+  (prs : fmap var (state -> Prop)) x b st st' pm,
+  (forall x b, pm $? x = Some b
+       -> match prs $? x with
+          | Some pr => pr st <-> b = true
+          | None => False
+          end)
+  -> doIt st st'
+  -> forall rs pm', (forall r, In r rs -> ruleAccurate prs doIt r)
+  -> applyRules pm pm' rs $? x = Some b
+  -> (forall x b, pm' $? x = Some b
+                  -> match prs $? x with
+                     | None => False
+                     | Some pr => pr st' <-> b = true
+                     end)
+  -> match prs $? x with
+     | None => False
+     | Some pr => pr st' <-> b = true
+     end.
+Proof.
+  induct rs; simplify.
+
+  apply H3.
+  assumption.
+
+  eapply IHrs; simplify.
+  apply H1.
+  propositional.
+  eassumption.
+  eapply applyRule_sound.
+  apply H.
+  eassumption.
+  eassumption.
+  apply H1; propositional.
+  assumption.
+Qed.
+
+Theorem applyRules_sound : forall state (doIt : state -> state -> Prop)
+  (prs : fmap var (state -> Prop)) x b st st' rs pm,
+  (forall r, In r rs -> ruleAccurate prs doIt r)
+  -> (forall x b, pm $? x = Some b
+       -> match prs $? x with
+          | Some pr => pr st <-> b = true
+          | None => False
+          end)
+  -> applyRules pm $0 rs $? x = Some b
+  -> doIt st st'
+  -> match prs $? x with
+     | None => False
+     | Some pr => pr st' <-> b = true
+     end.
+Proof.
+  simplify.
+  eapply applyRules_sound'.
+  eassumption.
+  eassumption.
+  eassumption.
+  eassumption.
+  simplify.
+  equality.
+Qed.
+
+Theorem predicate_abstraction_simulates : forall pc state action
+  (pc0 : pc) (st0 : state)
+  (actionOf : pc -> action -> pc -> Prop)
+  (doAction : action -> state -> state -> Prop)
+  (pa : predicate_abstraction state action),
+  predicate_abstraction_sound doAction pa
+  -> simulates (paR pa)
+               (actionSys pc0 st0 actionOf doAction)
+               (predicate_abstract pc0 actionOf pa).
+Proof.
+  constructor; simplify.
+
+  propositional; subst.
+  exists (pc0, $0); propositional.
+  constructor; simplify.
+  equality.
+
+  invert H1.
+  invert H0.
+  exists (pc2, match pa.(Rules) $? act with
+               | None => $0
+               | Some rs => applyRules pm $0 rs
+               end); propositional.
+  constructor; simplify.
+  unfold predicate_abstraction_sound in H.
+  cases (Rules pa $? act); simplify; try equality.
+  eapply applyRules_sound.
+  simplify.
+  eapply H.
+  eassumption.
+  eassumption.
+  eassumption.
+  assumption.
+  assumption.
+
+  constructor; assumption.
+Qed.
+
+
+(* Optional part: using predicate abstraction for another example *)
+
+Import Program2 ZArith.
+
+
+Definition tr := {|AssumedPredicate := "np = npo";
+                   AssumedToBe := true|}.
+Definition fa := {|AssumedPredicate := "np = npo";
+                   AssumedToBe := false|}.
+
+Definition establish := [{|Assumptions := []; Conclusion := tr |}].
+Definition preserve := [{|Assumptions := [tr]; Conclusion := tr |};
+                         {|Assumptions := [fa]; Conclusion := fa |}].
+Definition falsify := [{|Assumptions := [tr]; Conclusion := fa |}].
+
+Definition locked := {|AssumedPredicate := "locked";
+                       AssumedToBe := true|}.
+Definition unlocked := {|AssumedPredicate := "locked";
+                         AssumedToBe := false|}.
+Definition take_lock := [{|Assumptions := []; Conclusion := locked |}].
+Definition release_lock := [{|Assumptions := []; Conclusion := unlocked |}].
+Definition preserve_lock := [{|Assumptions := [locked]; Conclusion := locked |};
+                              {|Assumptions := [unlocked]; Conclusion := unlocked |}].
+Definition while_false := [{|Assumptions := [fa]; Conclusion := locked |};
+                            {|Assumptions := [tr; locked]; Conclusion := locked |}].
+
+Definition sys_pa : predicate_abstraction state action := {|
+  Predicates := $0 $+ ("np = npo", fun st => st.(NP) = st.(NPO))
+                   $+ ("locked", fun st => st.(HasLock) = true);
+  Rules := $0 $+ (LockOK, preserve ++ take_lock)
+              $+ (AssignA, establish ++ preserve_lock)
+              $+ (IfFalse, preserve ++ preserve_lock)
+              $+ (IfTrue, preserve ++ preserve_lock)
+              $+ (UnlockOK, preserve ++ release_lock)
+              $+ (IncA, falsify ++ preserve_lock)
+              $+ (WhileFalse, while_false)
+              $+ (WhileTrue, preserve ++ preserve_lock)
+|}.
+
+Opaque Zplus.
+
+Theorem sys_ok : forall np npo,
+  invariantFor (sys np npo) (fun st => fst st = Unlock2 -> (snd st).(HasLock) = true).
+Proof.
+  simplify.
+  eapply invariant_weaken.
+  eapply invariant_simulates.
+  eapply predicate_abstraction_simulates with (pa := sys_pa).
+
+  unfold predicate_abstraction_sound; simplify.
+  cases act; simplify; invert H; unfold ruleAccurate, assertionAccurate in *; simplify; propositional; subst;
+    simplify; unfold assertionAccurate in *; simplify; propositional;
+    invert H1; simplify; propositional; equality || (try linear_arithmetic).
+
+  model_check_infer.
+
+  simplify.
+  invert H.
+  simplify.
+  propositional; subst; invert H1; simplify; try equality.
+  specialize (H3 "locked" true); simplify.
+  cases (HasLock st); propositional; equality.
+Qed.
