pset4/Pset4.v
@@ -8,18 +8,175 @@ Require Import Frap Pset4Sig.
 Section env.
 
   Variable env : environment.
-  
+  Hint Constructors trc step eval.
+
+  Lemma step_star_Seq : forall v c1 c2 v' c1',
+        (step env)^* (v, c1) (v', c1')
+        -> (step env)^* (v, Sequence c1 c2) (v', Sequence c1' c2).
+    Proof.
+      induct 1; eauto.
+      cases y; eauto.
+    Qed.
+
+  Hint Resolve step_star_Seq.
+
+  Lemma step_star_InCall : forall v c v' c' v0 lhs ret,
+        (step env)^* (v, c) (v', c')
+        -> (step env)^* (v, InCall v0 lhs ret c) (v', InCall v0 lhs ret c').
+  Proof.
+      induct 1; eauto.
+      cases y; eauto.
+  Qed.
+
+  Hint Resolve step_star_InCall.
+
+  Lemma step_star_Try : forall v c v' c' x handler,
+                          (step env) ^* (v, c) (v', c')
+                          (*-> (step env) ^* (v, Try c x handler) (v', c') \/
+                             (step env) ^* (v, Try c x handler) (v $+ (x, exn), handler).*)
+                          (*-> (step env) ^* (v, Try Skip x handler) (v, Skip) \/ *)
+                          -> (step env)^* (v, Try c x handler) (v', Try c' x handler).
+  Proof.
+    induct 1; eauto.
+    cases y; eauto.
+  Qed.
+
+  Hint Resolve step_star_Try.
+(*
+  Lemma step_star_TryDone : forall v x handler,
+                              (step env) ^* (v, Try Skip x handler) (v, Skip).
+  Proof.
+    econstructor; eauto.
+  Qed.
+
+  Hint Resolve step_star_TryDone.
+
+  Lemma step_star_TryThrow : forall v (n : nat) x handler,
+                               (step env)^* (v, Try (Throw (Const n)) x handler) (v $+ (x, n), handler).
+  Proof.
+    econstructor; eauto.
+  Qed.
+
+
+  Hint Resolve step_star_TryThrow.*)
+                              
   Theorem big_small : forall v c v',
       eval env v c (Normal, v')
       -> (step env)^* (v, c) (v', Skip).
   Proof.
+    
+    induct 1; simplify; eauto 5 using trc_trans.
+    {
+    econstructor.
+    eauto.
+    eapply trc_trans.
+    apply step_star_Seq.
+    eassumption.
+    eauto.
+    }
+    {
+    econstructor; eauto.
+    eapply trc_trans.
+     {
+      apply step_star_InCall.
+      eassumption.
+     }
+    eauto.
+    }
+    {
+      eapply trc_trans.
+      {
+        apply step_star_Try.
+        eauto.
+      }  
+      {
+        econstructor.
+        apply StepTry.
+        
+        
+        
+        
+        
+        
+        
+      (*
+      {
+        apply step_star_Try.
+        eauto.
+      }
+      {
+        econstructor;eauto.
+        apply step_star_TryThrow.
+      }
+      {
+        econstructor; eauto.
+        *)
+      
+  (*
+      assert (eval env v (Try c x handler) (Normal, v')).
+      exact (EvalTryExn env v c exn v'0  x handler (Normal, v') H H0).
+      cases c.
+      invert H.
+      invert H1.
+      invert H.
+      invert H.
+      
+      admit. (* sequence c1 c2 *)
+      admit.
+      admit.
+      admit.
+      admit.
+      admit.
+      
+      
+      Econstructor; eauto.
+      cases c.
+      econstructor; eauto.
+      econstructor; eauto.
+      SearchAbout trc.
+      trc_trans      
+      econstructor; eauto.
+      cases c.
+      *)
+        
+    
+    
   Admitted.
+
+
 
   Theorem big_small_exn : forall v c n v',
       eval env v c (Exception n, v')
       -> (step env)^* (v, c) (v', Throw (Const n)).
   Proof.
   Admitted.
+
+  Lemma small_big'' : forall v c v' c',
+        (step env) (v, c) (v', c')
+        -> forall v'', eval v' c' v''
+                       -> eval v c v''.
+    Proof.
+      induct 1; simplify;
+        repeat match goal with
+               | [ H : eval _ _ _ |- _ ] => invert1 H
+               end; eauto.
+      {
+        econstructor; eauto.
+      }
+    Qed.
+
+    Hint Resolve small_big''.
+
+    Lemma small_big' : forall v c v' c',
+        (step env)^* (v, c) (v', c')
+        -> forall v'', eval v' c' v''
+                       -> eval v c v''.
+    Proof.
+      induct 1; eauto.
+      cases y; eauto.
+    Qed.
+
+    Hint Resolve small_big'.
 
   Theorem small_big : forall v c v',
       (step env)^* (v, c) (v', Skip)
